holsrcs/statesScript.sml
@@ -98,9 +98,13 @@ val _ = Hol_datatype
                             variables can be references, and these can be
                             (initialised to be) references to sub-classes. *)
 
-              thisvalue: CExpr option
+              thisvalue: CExpr option ;
                          (* the value (i.e., this will always be an ECompVal
                             with a pointer value) of the this expression *)
+
+              constructors: string # CPP_Type list |-> fn_info
+                         (* constructor information per class name and
+                            parameter types *)
              |>`;
 val _ = type_abbrev("CState", ``:state``)
 
